Integrating

src/asn1/RIoT.X509.Extension.fst
@@ -4,34 +4,79 @@ open ASN1.Spec
 open X509.BasicFields.Extension
 open RIoT.X509.CompositeDeviceID
 
+// #set-options "--z3rlimit 8"
+let _ = assert (length_of_oid OID_EC_GRP_SECP256R1 == 6)
+let _ = assert (length_of_asn1_primitive_TLV (Mkbit_string_t 33ul 0ul (magic())) == 35)
+
 unfold
 let riot_extension_t
-= x509_extension_t serialize_compositeDeviceID_sequence_TLV
+= x509_extension_t OID_RIOT serialize_compositeDeviceID_sequence_TLV
 
+unfold
 let parse_riot_extension
 : parser parse_x509_extension_kind riot_extension_t
-= parse_x509_extension serialize_compositeDeviceID_sequence_TLV
+= parse_x509_extension OID_RIOT serialize_compositeDeviceID_sequence_TLV
 
+unfold
 let serialize_riot_extension
 : serializer parse_riot_extension
-= serialize_x509_extension serialize_compositeDeviceID_sequence_TLV
+= serialize_x509_extension OID_RIOT serialize_compositeDeviceID_sequence_TLV
+
+#set-options "--z3rlimit 8"
+let _ = assert (length_of_oid OID_EC_GRP_SECP256R1 == 6)
+let _ = assert (length_of_asn1_primitive_TLV (Mkbit_string_t 33ul 0ul (magic())) == 35)
+
+let lemma_serialize_riot_extension_unfold
+= lemma_serialize_x509_extension_unfold OID_RIOT serialize_compositeDeviceID_sequence_TLV
+
+let lemma_serialize_riot_extension_size
+= lemma_serialize_x509_extension_size OID_RIOT serialize_compositeDeviceID_sequence_TLV
 
 
 let riot_extension_t_inbound
-= x509_extension_t_inbound serialize_compositeDeviceID_sequence_TLV
+= x509_extension_t_inbound OID_RIOT serialize_compositeDeviceID_sequence_TLV
 
 let parse_riot_extension_sequence_TLV
 : parser parse_x509_extension_sequence_TLV_kind riot_extension_t_inbound
-= assert (x509_extension_t_inbound serialize_compositeDeviceID_sequence_TLV == riot_extension_t_inbound);
+= assert (x509_extension_t_inbound OID_RIOT serialize_compositeDeviceID_sequence_TLV == riot_extension_t_inbound);
   riot_extension_t_inbound
   `coerce_parser`
-  parse_x509_extension_sequence_TLV serialize_compositeDeviceID_sequence_TLV
+  parse_x509_extension_sequence_TLV OID_RIOT serialize_compositeDeviceID_sequence_TLV
 
 let serialize_riot_extension_sequence_TLV
 : serializer parse_riot_extension_sequence_TLV
-= serialize_x509_extension_sequence_TLV serialize_compositeDeviceID_sequence_TLV
+= coerce_parser_serializer
+  (* p2 *) parse_riot_extension_sequence_TLV
+  (* s1 *) (serialize_x509_extension_sequence_TLV OID_RIOT serialize_compositeDeviceID_sequence_TLV)
+  (* prf*) ()
 
-(*)
-let serialize_riot_extension_sequence_TLV
-: serializer parse_riot_extension_sequence_TLV
-= serialize_x509_extension_sequence_TLV serialize_x509_extension_sequence_TLV
+let lemma_serialize_riot_extension_sequence_TLV_unfold
+= lemma_serialize_x509_extension_sequence_TLV_unfold OID_RIOT serialize_compositeDeviceID_sequence_TLV
+
+let lemma_serialize_riot_extension_sequence_TLV_size
+= lemma_serialize_x509_extension_sequence_TLV_size OID_RIOT serialize_compositeDeviceID_sequence_TLV
+
+(* low *)
+open ASN1.Low
+
+let serialize32_riot_extension_backwards
+: serializer32_backwards serialize_riot_extension
+= coerce_serializer32_backwards
+  (* s2 *) (serialize_riot_extension)
+  (* s32*) (serialize32_x509_extension_backwards
+              OID_RIOT
+              serialize32_compositeDeviceID_sequence_TLV_backwards)
+  (* prf*) ()
+
+let serialize32_riot_extension_sequence_TLV_backwards
+= coerce_serializer32_backwards
+  (* s2 *) (serialize_riot_extension_sequence_TLV)
+  (* s32*) (serialize32_x509_extension_sequence_TLV_backwards
+              OID_RIOT
+              serialize32_compositeDeviceID_sequence_TLV_backwards)
+  (* prf*) ()
+
+
+#set-options "--z3rlimit 8"
+let _ = assert (length_of_oid OID_EC_GRP_SECP256R1 == 6)
+let _ = assert (length_of_asn1_primitive_TLV (Mkbit_string_t 33ul 0ul (magic())) == 35)
